rt haskell+refine: more uniformly handle endpoint and notification queues
- Introduce functions to append and dequeue to/from endpoint and notification
  queues, in order to make verification feasible. Handle linked list
  manipulations with the same functions that were previously used for the
  ready and release queues, together with the new function orderedInsert for
  inserting a pointer into a list.

  Use only the fields tcbSchedNext and tcbSchedPrev for the endpoint,
  notification, ready, and release queues, since any thread can be in at most
  one of these queues at a time.

- Introduce heap_pspace_relation and heap_ghost_relation so that the
  conjuncts in state_relation can be expressed in terms of minimal heaps.
  Give lifting rules for rcorres for these two new predicates as well as the
  other conjuncts in state_relation.

- Modify the definitions of cancelAllIPC and cancelAllSignals to dequeue the
  head of the list during each iteration of the loop, in order to align with
  the C.

Signed-off-by: Michael McInerney <michael.mcinerney@proofcraft.systems>

spec/haskell/src/SEL4/Object/ObjectType.lhs
@@ -171,6 +171,7 @@ Threads are treated as special capability nodes; they also become zombies when t
 >     return (Zombie cte_ptr ZombieTCB 5, NullCap)
 
 > finaliseCap (SchedContextCap { capSchedContextPtr = scPtr }) True _ = do
+>     stateAssert sch_act_simple_asrt "`sch_act_simple` must hold"
 >     schedContextUnbindAllTCBs scPtr
 >     schedContextUnbindNtfn scPtr
 >     schedContextUnbindReply scPtr
